Instead of using option, use a Fetch to keep track of missing values

Ext2.v
@@ -1,8 +1,9 @@
 Require Import Coq.ZArith.ZArith.
 
 Require Import ByteData.
-Require Import Util.
+Require Import Fetch.
 Require Import File.
+Require Import Util.
 
 Open Local Scope Z.
 
@@ -66,53 +67,53 @@ Structure SuperBlock := mkSuperBlock {
   firstMetaBg: Z
 }.
 
-Definition findAndParseSuperBlock (disk: Disk): Exc SuperBlock :=
+Definition findAndParseSuperBlock (disk: Disk): @Fetch SuperBlock :=
   let disk := (shift disk 1024) in
-  (seq_lendu disk 0 4) _flatmap_ (fun inodesCount =>
-  (seq_lendu disk 4 4) _flatmap_ (fun blocksCount =>
-  (seq_lendu disk 8 4) _flatmap_ (fun rBlocksCount =>
-  (seq_lendu disk 12 4) _flatmap_ (fun freeBlocksCount =>
-  (seq_lendu disk 16 4) _flatmap_ (fun freeInodesCount =>
-  (seq_lendu disk 20 4) _flatmap_ (fun firstDataBlock =>
-  (seq_lendu disk 24 4) _flatmap_ (fun logBlockSize =>
-  (seq_lendu disk 28 4) _flatmap_ (fun logFragSize =>
-  (seq_lendu disk 32 4) _flatmap_ (fun blocksPerGroup =>
-  (seq_lendu disk 36 4) _flatmap_ (fun fragsPerGroup =>
-  (seq_lendu disk 40 4) _flatmap_ (fun inodesPerGroup =>
-  (seq_lendu disk 44 4) _flatmap_ (fun mTime =>
-  (seq_lendu disk 48 4) _flatmap_ (fun wTime =>
-  (seq_lendu disk 52 2) _flatmap_ (fun mntCount =>
-  (seq_lendu disk 54 2) _flatmap_ (fun maxMntCount =>
-  (seq_lendu disk 56 2) _flatmap_ (fun magic =>
-  (seq_lendu disk 58 2) _flatmap_ (fun state =>
-  (seq_lendu disk 60 2) _flatmap_ (fun errors =>
-  (seq_lendu disk 62 2) _flatmap_ (fun minorRevLevel =>
-  (seq_lendu disk 64 4) _flatmap_ (fun lastCheck =>
-  (seq_lendu disk 68 4) _flatmap_ (fun checkinterval =>
-  (seq_lendu disk 72 4) _flatmap_ (fun creatorOS =>
-  (seq_lendu disk 76 4) _flatmap_ (fun revLevel =>
-  (seq_lendu disk 80 2) _flatmap_ (fun defResuid =>
-  (seq_lendu disk 82 2) _flatmap_ (fun defResgid =>
-  (seq_lendu disk 84 4) _flatmap_ (fun firstIno =>
-  (seq_lendu disk 88 2) _flatmap_ (fun inodeSize =>
-  (seq_lendu disk 90 2) _flatmap_ (fun blockGroupNr =>
-  (seq_lendu disk 92 4) _flatmap_ (fun featureCompat =>
-  (seq_lendu disk 96 4) _flatmap_ (fun featureIncompat =>
-  (seq_lendu disk 100 4) _flatmap_ (fun featureROCompat =>
-  (seq_list disk 104 16) _flatmap_ (fun uuid =>
-  (seq_list disk 120 16) _flatmap_ (fun volumeName =>
-  (seq_list disk 136 64) _flatmap_ (fun lastMounted =>
-  (seq_lendu disk 200 4) _flatmap_ (fun algoBitmap =>
-  (disk 204) _flatmap_ (fun preallocBlocks =>
-  (disk 205) _flatmap_ (fun preallocDirBlocks =>
-  (seq_lendu disk 208 16) _flatmap_ (fun journalUUID =>
-  (seq_lendu disk 224 4) _flatmap_ (fun journalInum =>
-  (seq_lendu disk 228 4) _flatmap_ (fun journalDev =>
-  (seq_lendu disk 232 4) _flatmap_ (fun lastOrphan =>
-  (seq_lendu disk 236 16) _flatmap_ (fun hashSeed =>
-  (disk 252) _flatmap_ (fun defHashVersion =>
-  (seq_lendu disk 256 4) _flatmap_ (fun defaultMountOptions =>
-  (seq_lendu disk 260 4) _map_ (fun firstMetaBg =>
+  (seq_lendu disk 0 4) _fflatmap_ (fun inodesCount =>
+  (seq_lendu disk 4 4) _fflatmap_ (fun blocksCount =>
+  (seq_lendu disk 8 4) _fflatmap_ (fun rBlocksCount =>
+  (seq_lendu disk 12 4) _fflatmap_ (fun freeBlocksCount =>
+  (seq_lendu disk 16 4) _fflatmap_ (fun freeInodesCount =>
+  (seq_lendu disk 20 4) _fflatmap_ (fun firstDataBlock =>
+  (seq_lendu disk 24 4) _fflatmap_ (fun logBlockSize =>
+  (seq_lendu disk 28 4) _fflatmap_ (fun logFragSize =>
+  (seq_lendu disk 32 4) _fflatmap_ (fun blocksPerGroup =>
+  (seq_lendu disk 36 4) _fflatmap_ (fun fragsPerGroup =>
+  (seq_lendu disk 40 4) _fflatmap_ (fun inodesPerGroup =>
+  (seq_lendu disk 44 4) _fflatmap_ (fun mTime =>
+  (seq_lendu disk 48 4) _fflatmap_ (fun wTime =>
+  (seq_lendu disk 52 2) _fflatmap_ (fun mntCount =>
+  (seq_lendu disk 54 2) _fflatmap_ (fun maxMntCount =>
+  (seq_lendu disk 56 2) _fflatmap_ (fun magic =>
+  (seq_lendu disk 58 2) _fflatmap_ (fun state =>
+  (seq_lendu disk 60 2) _fflatmap_ (fun errors =>
+  (seq_lendu disk 62 2) _fflatmap_ (fun minorRevLevel =>
+  (seq_lendu disk 64 4) _fflatmap_ (fun lastCheck =>
+  (seq_lendu disk 68 4) _fflatmap_ (fun checkinterval =>
+  (seq_lendu disk 72 4) _fflatmap_ (fun creatorOS =>
+  (seq_lendu disk 76 4) _fflatmap_ (fun revLevel =>
+  (seq_lendu disk 80 2) _fflatmap_ (fun defResuid =>
+  (seq_lendu disk 82 2) _fflatmap_ (fun defResgid =>
+  (seq_lendu disk 84 4) _fflatmap_ (fun firstIno =>
+  (seq_lendu disk 88 2) _fflatmap_ (fun inodeSize =>
+  (seq_lendu disk 90 2) _fflatmap_ (fun blockGroupNr =>
+  (seq_lendu disk 92 4) _fflatmap_ (fun featureCompat =>
+  (seq_lendu disk 96 4) _fflatmap_ (fun featureIncompat =>
+  (seq_lendu disk 100 4) _fflatmap_ (fun featureROCompat =>
+  (seq_list disk 104 16) _fflatmap_ (fun uuid =>
+  (seq_list disk 120 16) _fflatmap_ (fun volumeName =>
+  (seq_list disk 136 64) _fflatmap_ (fun lastMounted =>
+  (seq_lendu disk 200 4) _fflatmap_ (fun algoBitmap =>
+  (disk 204) _fflatmap_ (fun preallocBlocks =>
+  (disk 205) _fflatmap_ (fun preallocDirBlocks =>
+  (seq_lendu disk 208 16) _fflatmap_ (fun journalUUID =>
+  (seq_lendu disk 224 4) _fflatmap_ (fun journalInum =>
+  (seq_lendu disk 228 4) _fflatmap_ (fun journalDev =>
+  (seq_lendu disk 232 4) _fflatmap_ (fun lastOrphan =>
+  (seq_lendu disk 236 16) _fflatmap_ (fun hashSeed =>
+  (disk 252) _fflatmap_ (fun defHashVersion =>
+  (seq_lendu disk 256 4) _fflatmap_ (fun defaultMountOptions =>
+  (seq_lendu disk 260 4) _fmap_ (fun firstMetaBg =>
     mkSuperBlock
       inodesCount
       blocksCount
@@ -180,7 +181,7 @@ Structure GroupDescriptor := mkGroupDescriptor {
 
 Definition findAndParseGroupDescriptor 
   (disk: Disk) (superblock: SuperBlock) (groupId: Z)
-  : Exc GroupDescriptor :=
+  : @Fetch GroupDescriptor :=
   let groupBlockArrayBA := if (blockSize superblock >? 1024)
     then 1 else 2 in
   let groupBlockArrayOffset :=
@@ -188,12 +189,12 @@ Definition findAndParseGroupDescriptor
   let descriptorOffset := 32 * groupId in
   let disk := (shift disk (groupBlockArrayOffset
                            + descriptorOffset)) in
-  (seq_lendu disk 0 4) _flatmap_ (fun blockBitmap =>
-  (seq_lendu disk 4 4) _flatmap_ (fun inodeBitmap =>
-  (seq_lendu disk 8 4) _flatmap_ (fun inodeTable =>
-  (seq_lendu disk 12 2) _flatmap_ (fun gdFreeBlocksCount =>
-  (seq_lendu disk 14 2) _flatmap_ (fun gdFreeInodesCount =>
-  (seq_lendu disk 16 2) _map_ (fun usedDirsCount =>
+  (seq_lendu disk 0 4) _fflatmap_ (fun blockBitmap =>
+  (seq_lendu disk 4 4) _fflatmap_ (fun inodeBitmap =>
+  (seq_lendu disk 8 4) _fflatmap_ (fun inodeTable =>
+  (seq_lendu disk 12 2) _fflatmap_ (fun gdFreeBlocksCount =>
+  (seq_lendu disk 14 2) _fflatmap_ (fun gdFreeInodesCount =>
+  (seq_lendu disk 16 2) _fmap_ (fun usedDirsCount =>
     mkGroupDescriptor
       blockBitmap
       inodeBitmap
@@ -228,10 +229,10 @@ Structure Inode := mkInode {
 
 Definition findAndParseInode (disk: Disk)
   (superblock: SuperBlock) (groupdesc: GroupDescriptor)
-  (inodeIndex: Z): Exc Inode :=
+  (inodeIndex: Z): @Fetch Inode :=
   (* Check for valid Inode *)
   if (inodeIndex >=? superblock.(inodesCount))
-  then error
+  then ErrorString "Invalid inode index"
   else
     (* Inode Table is 1-indexed *)
     let inodeIndexInTable := 
@@ -240,38 +241,38 @@ Definition findAndParseInode (disk: Disk)
                                groupdesc.(inodeTable))
                      + (inodeIndexInTable * 128) in
     let disk := (shift disk inodePos) in
-    (seq_lendu disk 0 2) _flatmap_ (fun mode =>
-    (seq_lendu disk 2 2) _flatmap_ (fun uid =>
-    (seq_lendu disk 4 4) _flatmap_ (fun size =>
-    (seq_lendu disk 8 4) _flatmap_ (fun atime =>
-    (seq_lendu disk 12 4) _flatmap_ (fun ctime =>
-    (seq_lendu disk 16 4) _flatmap_ (fun mtime =>
-    (seq_lendu disk 20 4) _flatmap_ (fun dtime =>
-    (seq_lendu disk 24 2) _flatmap_ (fun gid =>
-    (seq_lendu disk 26 2) _flatmap_ (fun linksCount =>
-    (seq_lendu disk 28 4) _flatmap_ (fun blocks =>
-    (seq_lendu disk 32 4) _flatmap_ (fun flags =>
-    (seq_lendu disk 36 4) _flatmap_ (fun osd1 =>
-    (seq_lendu disk 40 4) _flatmap_ (fun directBlock1 =>
-    (seq_lendu disk 44 4) _flatmap_ (fun directBlock2 =>
-    (seq_lendu disk 48 4) _flatmap_ (fun directBlock3 =>
-    (seq_lendu disk 52 4) _flatmap_ (fun directBlock4 =>
-    (seq_lendu disk 56 4) _flatmap_ (fun directBlock5 =>
-    (seq_lendu disk 60 4) _flatmap_ (fun directBlock6 =>
-    (seq_lendu disk 64 4) _flatmap_ (fun directBlock7 =>
-    (seq_lendu disk 68 4) _flatmap_ (fun directBlock8 =>
-    (seq_lendu disk 72 4) _flatmap_ (fun directBlock9 =>
-    (seq_lendu disk 76 4) _flatmap_ (fun directBlock10 =>
-    (seq_lendu disk 80 4) _flatmap_ (fun directBlock11 =>
-    (seq_lendu disk 84 4) _flatmap_ (fun directBlock12 =>
-    (seq_lendu disk 88 4) _flatmap_ (fun indirectBlock =>
-    (seq_lendu disk 92 4) _flatmap_ (fun doubleIndirectBlock =>
-    (seq_lendu disk 96 4) _flatmap_ (fun tripleIndirectBlock =>
-    (seq_lendu disk 100 4) _flatmap_ (fun generation =>
-    (seq_lendu disk 104 4) _flatmap_ (fun fileACL =>
-    (seq_lendu disk 108 4) _flatmap_ (fun dirACL =>
-    (seq_lendu disk 112 4) _flatmap_ (fun faddr =>
-    (seq_lendu disk 116 4) _map_ (fun osd2 =>
+    (seq_lendu disk 0 2) _fflatmap_ (fun mode =>
+    (seq_lendu disk 2 2) _fflatmap_ (fun uid =>
+    (seq_lendu disk 4 4) _fflatmap_ (fun size =>
+    (seq_lendu disk 8 4) _fflatmap_ (fun atime =>
+    (seq_lendu disk 12 4) _fflatmap_ (fun ctime =>
+    (seq_lendu disk 16 4) _fflatmap_ (fun mtime =>
+    (seq_lendu disk 20 4) _fflatmap_ (fun dtime =>
+    (seq_lendu disk 24 2) _fflatmap_ (fun gid =>
+    (seq_lendu disk 26 2) _fflatmap_ (fun linksCount =>
+    (seq_lendu disk 28 4) _fflatmap_ (fun blocks =>
+    (seq_lendu disk 32 4) _fflatmap_ (fun flags =>
+    (seq_lendu disk 36 4) _fflatmap_ (fun osd1 =>
+    (seq_lendu disk 40 4) _fflatmap_ (fun directBlock1 =>
+    (seq_lendu disk 44 4) _fflatmap_ (fun directBlock2 =>
+    (seq_lendu disk 48 4) _fflatmap_ (fun directBlock3 =>
+    (seq_lendu disk 52 4) _fflatmap_ (fun directBlock4 =>
+    (seq_lendu disk 56 4) _fflatmap_ (fun directBlock5 =>
+    (seq_lendu disk 60 4) _fflatmap_ (fun directBlock6 =>
+    (seq_lendu disk 64 4) _fflatmap_ (fun directBlock7 =>
+    (seq_lendu disk 68 4) _fflatmap_ (fun directBlock8 =>
+    (seq_lendu disk 72 4) _fflatmap_ (fun directBlock9 =>
+    (seq_lendu disk 76 4) _fflatmap_ (fun directBlock10 =>
+    (seq_lendu disk 80 4) _fflatmap_ (fun directBlock11 =>
+    (seq_lendu disk 84 4) _fflatmap_ (fun directBlock12 =>
+    (seq_lendu disk 88 4) _fflatmap_ (fun indirectBlock =>
+    (seq_lendu disk 92 4) _fflatmap_ (fun doubleIndirectBlock =>
+    (seq_lendu disk 96 4) _fflatmap_ (fun tripleIndirectBlock =>
+    (seq_lendu disk 100 4) _fflatmap_ (fun generation =>
+    (seq_lendu disk 104 4) _fflatmap_ (fun fileACL =>
+    (seq_lendu disk 108 4) _fflatmap_ (fun dirACL =>
+    (seq_lendu disk 112 4) _fflatmap_ (fun faddr =>
+    (seq_lendu disk 116 4) _fmap_ (fun osd2 =>
       mkInode
         mode
         uid
@@ -303,7 +304,7 @@ Definition findAndParseInode (disk: Disk)
 (* Recursive function for dealing with levels of indirection *)
 Fixpoint walkIndirection (disk: Disk) (superblock: SuperBlock)
   (blockNumber indirectionPos: Z) (indirectionLevel: nat) 
-  : Exc Z :=
+  : @Fetch Z :=
   match indirectionLevel with
   | O => 
       let bytePosition := (indirectionPos + 4 * blockNumber) in
@@ -317,7 +318,7 @@ Fixpoint walkIndirection (disk: Disk) (superblock: SuperBlock)
     let nextBytePosition := 
       indirectionPos + 4 * nextBlockIndex in
     (seq_lendu disk nextBytePosition 4) 
-      _flatmap_ (fun nextBlockBA =>
+      _fflatmap_ (fun nextBlockBA =>
       walkIndirection disk superblock 
                       (blockNumber mod unitSizeInBlocks)
                       (ba2Offset superblock nextBlockBA)
@@ -327,9 +328,9 @@ Fixpoint walkIndirection (disk: Disk) (superblock: SuperBlock)
 
 
 Definition fetchInodeByte (disk: Disk) (superblock: SuperBlock) 
-  (inode: Inode) (bytePos: Z): Exc Z :=
+  (inode: Inode) (bytePos: Z): @Fetch Z :=
   if inode.(size) <=? bytePos then 
-    error
+    MissingAt bytePos
   else 
     let blockSize := (blockSize superblock) in
     let blockNumInFile := bytePos / blockSize in
@@ -338,47 +339,53 @@ Definition fetchInodeByte (disk: Disk) (superblock: SuperBlock)
     let indirect2Addressable := (blockSize * blockSize) / 16 in
 
     (if blockNumInFile <=? directAddressable then
-      nth_error inode.(block) (Z.to_nat blockNumInFile)
+      match (nth_error inode.(block) (Z.to_nat blockNumInFile)) with
+      | error => ErrorString "Data block not present"
+      | value v => Found v
+      end
 
      else if blockNumInFile <=? directAddressable
                                 + indirect1Addressable then
-      (nth_error inode.(block) 12) 
-        _flatmap_ (fun indirectBlock =>
+      match (nth_error inode.(block) 12) with
+      | error => ErrorString "Indirection block not present"
+      | value indirectBlock => 
         walkIndirection disk superblock 
           (blockNumInFile - 12)
           (ba2Offset superblock indirectBlock) 
           O
-        )
+      end
 
     else if blockNumInFile <=? directAddressable
                                + indirect1Addressable
                                + indirect2Addressable then
-      (nth_error inode.(block) 13) 
-        _flatmap_ (fun doubleIndirectBlock =>
+      match (nth_error inode.(block) 13)  with
+      | error => ErrorString "Double indirection block not present"
+      | value doubleIndirectBlock =>
         walkIndirection disk superblock
           (blockNumInFile - 12 - (blockSize / 4)) 
           (ba2Offset superblock doubleIndirectBlock) 
           (S O)
-        )
+      end
 
     else 
-      (nth_error inode.(block) 14) 
-        _flatmap_ (fun tripleIndirectBlock =>
+      match (nth_error inode.(block) 14) with
+      | error => ErrorString "Triple indirection block not present"
+      | value tripleIndirectBlock =>
         walkIndirection disk superblock 
           (blockNumInFile - directAddressable
                           - indirect1Addressable
                           - indirect2Addressable)
           (ba2Offset superblock tripleIndirectBlock)
           (S (S O))
-      )
-    ) _flatmap_ (fun blockAddress =>
+      end
+    ) _fflatmap_ (fun blockAddress =>
       disk (blockSize * blockAddress + (bytePos mod blockSize))
     ).
 
 
 (* ======= Delete ======= *)
 Definition parseDeleted (disk: Disk) (superblock: SuperBlock)
-  (groupdesc: GroupDescriptor) (inodeIndex: Z) : Exc bool :=
+  (groupdesc: GroupDescriptor) (inodeIndex: Z) : @Fetch bool :=
   let inodeIndexInGroup := 
     (* 1-Indexed *)
     (inodeIndex - 1) mod superblock.(inodesPerGroup) in
@@ -386,38 +393,26 @@ Definition parseDeleted (disk: Disk) (superblock: SuperBlock)
     ba2Offset superblock groupdesc.(inodeBitmap) in
   (* Fetch the allocation byte for this inode *)
   (disk (bitmapStart + (inodeIndexInGroup / 8))) 
-    _map_ (fun allocationByte =>
+    _fmap_ (fun allocationByte =>
     (* The bit associated with this inode is 0 *)
     (negb (Z.testbit allocationByte
                      (inodeIndexInGroup mod 8)))
   ).
 
 
-(* ======= File ======= *)
-Fixpoint annoying (disk: Disk) (superblock: SuperBlock) (inode: Inode) 
-  (relevantBytes: list Z): Map_Z_Z := 
-  match relevantBytes with
-  | nil => MZ.empty Z
-  | headByte :: tail => match (fetchInodeByte disk superblock inode headByte) with
-    | value byte => (update (pair headByte byte)
-                            (annoying disk superblock inode tail))
-    | error => (annoying disk superblock inode tail)
-  end
-end.
-
 Definition findAndParseFile (disk: Disk) (inodeIndex: Z) 
-  : Exc File :=
-  (findAndParseSuperBlock disk) _flatmap_ (fun superblock =>
+  : @Fetch File :=
+  (findAndParseSuperBlock disk) _fflatmap_ (fun superblock =>
   let groupId := ((inodeIndex - 1) (* One-indexed *)
                   / superblock.(inodesPerGroup)) in
   let inodeIndexInGroup :=
     (inodeIndex - 1) mod superblock.(inodesPerGroup) in
   (findAndParseGroupDescriptor disk superblock groupId) 
-    _flatmap_ (fun groupdesc =>
+    _fflatmap_ (fun groupdesc =>
   (findAndParseInode disk superblock groupdesc inodeIndex)
-    _flatmap_ (fun inode =>
+    _fflatmap_ (fun inode =>
   (parseDeleted disk superblock groupdesc inodeIndex)
-    _map_ (fun deleted =>
+    _fmap_ (fun deleted =>
     mkFile
       (value inodeIndex)
       inode.(size)
