Fetch.v
@@ -1,0 +1,36 @@
+Require Import Coq.Strings.String.
+Require Import Coq.ZArith.ZArith.
+Require Export List.
+
+Inductive Fetch {A:Type}: Type :=
+  | Found: A -> Fetch
+  | MissingAt: Z -> Fetch
+  | ErrorString: string -> Fetch
+.
+
+(* Functional programming idioms *)
+Definition fetch_flatmap {A B:Type} (opt: @Fetch A) (fn: A -> @Fetch B)
+  : @Fetch B :=
+  match opt with
+    | Found a => fn a
+    | MissingAt pos => MissingAt pos
+    | ErrorString msg => ErrorString msg
+  end.
+
+Definition fetch_map {A B:Type} (opt: @Fetch A) (fn: A -> B)
+  : @Fetch B :=
+  match opt with
+    | Found a => Found (fn a)
+    | MissingAt pos => MissingAt pos
+    | ErrorString msg => ErrorString msg
+  end.
+
+Infix "_fflatmap_" := fetch_flatmap (at level 50).
+Infix "_fmap_" := fetch_map (at level 50).
+
+Fixpoint fetch_flatten {A} (lst: list (@Fetch A)): list A :=
+  match lst with
+    | (Found head) :: tail => head :: (fetch_flatten tail)
+    | _ :: tail => fetch_flatten tail
+    | nil => nil
+  end.
