FileSystems.v
@@ -2,6 +2,7 @@ Require Import Coq.ZArith.ZArith.
 
 Require Import ByteData.
 Require Import Ext2.
+Require Import Fetch.
 Require Import File.
 
 Open Local Scope Z.
@@ -11,13 +12,14 @@ Definition isOnDiskTry1 (file: File) (disk: Disk) :=
   (i >= 0 /\ i < file.(fileSize)) ->
     file @[ i ] = disk (start + i).
 
-Definition fileEq (lhs rhs: Exc File) :=
+Definition fileEq (lhs rhs: @Fetch File) :=
   match (lhs, rhs) with
-  | (error, error) => True
-  | (value lhs, value rhs) =>
+  | (Found lhs, Found rhs) =>
       lhs.(fileSize) = rhs.(fileSize)
       /\ lhs.(deleted) = rhs.(deleted)
       /\ forall idx:Z, lhs @[ idx ] = rhs @[ idx ]
+  | (ErrorString lhs, ErrorString rhs) => lhs = rhs
+  | (MissingAt lhs, MissingAt rhs) => lhs = rhs
   | _ => False
   end.
 
@@ -25,6 +27,6 @@ Definition isOnDisk (file: File) (disk: Disk) :=
   (* Ext2 *)
   (exists (inodeIndex: Z),
     fileEq (Ext2.findAndParseFile disk inodeIndex)
-           (value file))
+           (Found file))
   (* Disjunction with other file systems *)
 .
